DigitalObjects/TxLib.lean
@@ -1,3 +1,4 @@
 import DigitalObjects.TxLib.Events
 import DigitalObjects.TxLib.Predicates
 import DigitalObjects.TxLib.PredicatesSimpleProofs
+import DigitalObjects.TxLib.PredicatesSimple
